LeanPool/Lentil/ProofMode/Tactics/LeftRight.lean
@@ -14,24 +14,24 @@ section
 variable {σ : Type u} {hyps : List (NamedPred σ)} {a b : pred σ}
 
 -- NOTE: Implemented in a way that is probably more boring than you'd have expected
-theorem Entails_or_left : Entails hyps a → Entails hyps (tla_or a b) :=
+theorem Entails_or_left : Entails hyps a → Entails hyps (tlaOr a b) :=
   fun h => pred_implies_trans h TLA.or_inl
 
-theorem Entails_or_right : Entails hyps b → Entails hyps (tla_or a b) :=
+theorem Entails_or_right : Entails hyps b → Entails hyps (tlaOr a b) :=
   fun h => pred_implies_trans h TLA.or_inr
 
 end
 
 /--
-`tla_left` reduces a disjunctive proof-mode goal `p ∨ q` to its left disjunct
+`tlaLeft` reduces a disjunctive proof-mode goal `p ∨ q` to its left disjunct
 `p`.
 -/
-macro "tla_left" : tactic => `(tactic| refine $(mkIdent ``Entails_or_left) ?_)
+macro "tlaLeft" : tactic => `(tactic| refine $(mkIdent ``Entails_or_left) ?_)
 
 /--
-`tla_right` reduces a disjunctive proof-mode goal `p ∨ q` to its right
+`tlaRight` reduces a disjunctive proof-mode goal `p ∨ q` to its right
 disjunct `q`.
 -/
-macro "tla_right" : tactic => `(tactic| refine $(mkIdent ``Entails_or_right) ?_)
+macro "tlaRight" : tactic => `(tactic| refine $(mkIdent ``Entails_or_right) ?_)
 
 end TLA.ProofMode
