LeanPool/Lentil/ProofMode/Tactics/Start.lean
@@ -12,11 +12,11 @@ open Lean Meta Elab Tactic
 
 private def sequent? (e : Expr) : Option (Expr × Expr × Expr) :=
   match_expr e with
-  | TLA.pred_implies σ lhs rhs => some (σ, lhs, rhs)
+  | TLA.predImplies σ lhs rhs => some (σ, lhs, rhs)
   | _ => none
 
 private def getPremiseList (lhs : Expr) : MetaM (List Expr) := do
-  if lhs.isAppOfArity' ``TLA.tla_true 1 then pure [] else TLA.Expr.splitAndIntoParts lhs
+  if lhs.isAppOfArity' ``TLA.tlaTrue 1 then pure [] else TLA.Expr.splitAndIntoParts lhs
 
 private def mkNamedPredListExpr (σ : Expr) (hyps : List (String × Expr)) : MetaM Expr := do
   let elemTy ← mkAppM ``TLA.ProofMode.NamedPred #[σ]
