LeanPool/Lentil/Tactics/Basic.lean
@@ -17,39 +17,39 @@ macro_rules
   | `(tactic| try_unfold_at_all $idt:ident ) => `(tactic| (try unfold $idt at *) )
   | `(tactic| try_unfold_at_all $idt:ident $idts:ident* ) => `(tactic| (try unfold $idt at *); try_unfold_at_all $idts* )
 
-attribute [tlasimp_def] leads_to weak_fairness tla_and tla_or tla_not tla_implies tla_forall tla_exists tla_true tla_false always_implies
-  always eventually later tla_until state_pred pure_pred action_pred
-  valid pred_implies exec.satisfies exec.drop_drop
-  tla_bigwedge tla_bigvee Foldable.fold
+attribute [tlasimp_def] leadsTo weakFairness tlaAnd tlaOr tlaNot tlaImplies tlaForall tlaExists tlaTrue tlaFalse alwaysImplies
+  always eventually later tlaUntil statePred purePred actionPred
+  valid predImplies exec.satisfies exec.drop_drop
+  tlaBigwedge tlaBigvee Foldable.fold
 
 attribute [execsimp] exec.drop Nat.add_zero Nat.zero_add
 
 /-- Unfold TLA definitions in all hypotheses and the goal. -/
-macro "tla_unfold" : tactic => `(tactic| (try dsimp only [tlasimp_def] at *))
+macro "tlaUnfold" : tactic => `(tactic| (try dsimp only [tlasimp_def] at *))
 
 /-- Unfold TLA and execution definitions everywhere. -/
-macro "tla_unfold'" : tactic => `(tactic| (tla_unfold; (try dsimp only [execsimp] at *)))
+macro "tlaUnfold'" : tactic => `(tactic| (tlaUnfold; (try dsimp only [execsimp] at *)))
 
 /-- Unfold TLA definitions and simplify everywhere. -/
-macro "tla_unfold_simp" : tactic => `(tactic| (simp [tlasimp_def] at *))
+macro "tlaUnfoldSimp" : tactic => `(tactic| (simp [tlasimp_def] at *))
 
 /-- Unfold TLA and execution definitions and simplify everywhere. -/
-macro "tla_unfold_simp'" : tactic => `(tactic| (tla_unfold_simp; (try simp only [execsimp] at *)))
+macro "tlaUnfoldSimp'" : tactic => `(tactic| (tlaUnfoldSimp; (try simp only [execsimp] at *)))
 
-attribute [tla_nontemporal_def] tla_and tla_or tla_not tla_implies tla_forall tla_exists tla_true tla_false
-  state_pred pure_pred action_pred
-  valid pred_implies exec.satisfies
-  tla_bigwedge tla_bigvee Foldable.fold
+attribute [tla_nontemporal_def] tlaAnd tlaOr tlaNot tlaImplies tlaForall tlaExists tlaTrue tlaFalse
+  statePred purePred actionPred
+  valid predImplies exec.satisfies
+  tlaBigwedge tlaBigvee Foldable.fold
 
 /-- Simplify with the non-temporal TLA lemmas everywhere. -/
-macro "tla_nontemporal_simp" : tactic => `(tactic| (simp [tla_nontemporal_def] at *))
+macro "tlaNontemporalSimp" : tactic => `(tactic| (simp [tla_nontemporal_def] at *))
 
 /-- Normalize a sequent goal into a validity goal, by definitional equality. -/
 def changePredImpliesToValid : TacticM Unit := withMainContext do
   let target ← getMainTarget
   match_expr target.headBeta.cleanupAnnotations with
-  | TLA.pred_implies _ p q =>
-    let imp ← mkAppM ``TLA.tla_implies #[p, q]
+  | TLA.predImplies _ p q =>
+    let imp ← mkAppM ``TLA.tlaImplies #[p, q]
     let target' ← mkAppM ``TLA.valid #[imp]
     let goal ← getMainGoal
     replaceMainGoal [← goal.change target']
