LeanPool/Lentil/Util.lean
@@ -31,7 +31,7 @@ register_simp_attr tlasimp_def
 /-- Marking the things to simplify when explicitly reasoning about `exec`. -/
 register_simp_attr execsimp
 
-/-- Marking the definitions unfolded by `tla_finite_window`. -/
+/-- Marking the definitions unfolded by `tlaFiniteWindow`. -/
 register_simp_attr tla_finite_window_def
 
 /-- Marking the theorems that can be simplify reasoning at the TLA level. -/
